Changed my mind about ok_Bg representation

OkLib.v
@@ -1,13 +1,7 @@
+Require Import Setoid.
 Require Export Shared.
 Require Export PermutLib.
 Require Export PPermutLib.
-
-Require Export LibLogic.
-Require Export LibVar.
-Require Export LibList.
-Require Import Setoid.
-
-Require Export LibTactics. (* for skip *)
 
 Open Scope permut_scope.
 
@@ -16,19 +10,66 @@ Set Implicit Arguments.
 
 Section Definitions.
 
-Variable A: Type.
+Variables A B : Type.
 
-Fixpoint ok (G: list (var * A)) (Used: list var) : Prop :=
-match G with
-| nil => True
-| (w, Gamma) :: G => If Mem w Used then False else ok G (w::Used)
-end.
+Inductive ok_LF: list (var * A) -> list var -> Prop :=
+| ok_nil: forall U, ok_LF nil U
+| ok_step: forall w C G U,
+  ~ Mem w U -> ok_LF G (w::U) -> ok_LF ((w, C)::G) U
+.
+
+(* Copied from standard list, but this one uses List from LibList *)
+Definition flat_map (f:A -> list B) :=
+  fix flat_map (l:list A) : list B :=
+  match l with
+    | nil => nil
+    | x :: t => (f x)++(flat_map t)
+  end.
+
+Section FlatMapProp.
+
+Variable f : A -> list B.
+
+Lemma flat_map_nil :
+  flat_map f nil = nil.
+Proof. auto. Qed.
+
+Lemma flat_map_cons : forall x l,
+  flat_map f (x::l) = f x ++ flat_map f l.
+Proof. auto. Qed.
+
+Lemma flat_map_app : forall l1 l2,
+  flat_map f (l1 ++ l2) = flat_map f l1 ++ flat_map f l2.
+Admitted. (* !!! *)
+
+Lemma flat_map_last : forall x l,
+  flat_map f (l & x) = flat_map f l ++ f x.
+Proof. intros. rewrite flat_map_app; simpl; rew_app; auto. Qed.
+
+End FlatMapProp.
 
 End Definitions.
 
+Definition snd_ {A} {B} (p:A * B) :=
+  match p with
+  | (x, y) => y
+  end.
+
+Hint Rewrite flat_map_nil flat_map_cons flat_map_app flat_map_last :
+  rew_flat_map.
+
+Tactic Notation "rew_flat_map" :=
+  autorewrite with rew_flat_map rew_app.
+Tactic Notation "rew_flat_map" "in" hyp(H) :=
+  autorewrite with rew_flat_map rew_app in H.
+Tactic Notation "rew_flat_map" "in" "*" :=
+  autorewrite with rew_flat_map rew_app in *.
+
+
 Definition ok_Bg (G: Background_LF) : Prop :=
-ok G nil  /\
-ok (flat_map snd G) nil.
+ok_LF G nil  /\
+ok_LF (flat_map snd_ G) nil.
+
 
 Fixpoint used_t_vars (G: Background_LF) :=
 match G with
@@ -44,105 +85,106 @@ end.
 
 (*** Lemmas ***)
 
-(* ok for a generic type *)
+(* ok_LF for a generic type *)
 
-Lemma ok_used_permut:
+Lemma ok_LF_used_permut:
 forall A G U U',
   U *=* U' ->
-  (@ok A G U) ->
-  (@ok A G U').
+  (@ok_LF A G U) ->
+  (@ok_LF A G U').
+(*
 induction G; intros; simpl in *; auto.
-destruct a; repeat case_if.
+destruct a. repeat case_if.
 elim H2; apply Mem_permut with (l:=U'); [ symmetry | ]; auto.
 eapply IHG; eauto.
 Qed.
+*)Admitted.
 
-Lemma ok_used_weakening:
+Lemma ok_LF_used_weakening:
 forall A G x U,
-  (@ok A G (x::U)) ->
-  (@ok A G U).
-induction G; simpl; intros; auto;
+  (@ok_LF A G (x::U)) ->
+  (@ok_LF A G U).
+(*induction G; simpl; intros; auto;
 destruct a; repeat case_if.
 elim H1; rewrite Mem_cons_eq; right; auto.
 apply IHG with (x:=x).
-apply ok_used_permut with (U := (v::x::U));
-[ permut_simpl | auto].
-Qed.
+apply ok_LF_used_permut with (U := (v::x::U));
+[ permut_simpl | auto].*) Admitted.
 
-Lemma ok_split:
+Lemma ok_LF_split:
 forall A G1 G2 U,
-  (@ok A (G1++G2) U) ->
-  ok G1 U /\ ok G2 U.
-induction G1; intros; split; rew_app in *; simpl; auto;
+  (@ok_LF A (G1++G2) U) ->
+  ok_LF G1 U /\ ok_LF G2 U.
+(*induction G1; intros; split; rew_app in *; simpl; auto;
 destruct a; simpl in *; case_if.
 apply IHG1 with (G2:=G2); eauto.
-apply IHG1 with (G2:=G2); apply ok_used_weakening in H; eauto.
-Qed.
+apply IHG1 with (G2:=G2); apply ok_LF_used_weakening in H; eauto.
+Qed. *) Admitted.
 
-(* ok for a specific type -- would be nice to make it more general btw *)
+(* ok_LF for a specific type -- would be nice to make it more general btw *)
 
-Add Morphism (@ok (list (var*ty))) : ok_PPermut_lst_var_ty.
+Add Morphism (@ok_LF (list (var*ty))) : ok_LF_PPermut_lst_var_ty.
 Admitted. (* !!! *)
 
 (* FIXME: how to add this as morphism? *)
-Lemma ok_PPermut_ty:
+Lemma ok_LF_PPermut_ty:
 forall G G', G ~=~ G' ->
-  ok (flat_map snd G) nil ->
-  ok (flat_map snd G') nil.
+  ok_LF (flat_map snd_ G) nil ->
+  ok_LF (flat_map snd_ G') nil.
 Admitted. (* !!! *)
 
-Lemma ok_fresh_te_list:
+Lemma ok_LF_fresh_te_list:
 forall G Gamma v A w,
- ok ((w, Gamma) :: G) nil ->
+ ok_LF ((w, Gamma) :: G) nil ->
  v \notin (used_t_vars ((w,Gamma)::G)) ->
- ok ((w, (v,A)::Gamma) :: G) nil.
+ ok_LF ((w, (v,A)::Gamma) :: G) nil.
 Admitted. (* !!! *)
 
-Lemma ok_fresh_te_ty:
+Lemma ok_LF_fresh_te_ty:
 forall G Gamma v A w,
- ok (flat_map snd ((w, Gamma) :: G)) nil ->
+ ok_LF (flat_map snd_ ((w, Gamma) :: G)) nil ->
  v \notin (used_t_vars ((w,Gamma)::G)) ->
- ok (flat_map snd ((w, (v,A)::Gamma) :: G)) nil.
+ ok_LF (flat_map snd_ ((w, (v,A)::Gamma) :: G)) nil.
 Admitted. (* !!! *)
 
-Lemma ok_fresh_wo_list:
+Lemma ok_LF_fresh_wo_list:
 forall G v w,
- ok G nil ->
+ ok_LF G nil ->
  v \notin (used_w_vars G) ->
- ok ((w, nil) :: G) nil.
+ ok_LF ((w, nil) :: G) nil.
 Admitted. (* !!! *)
 
-Lemma ok_fresh_wo_ty:
+Lemma ok_LF_fresh_wo_ty:
 forall G v w,
- ok (flat_map snd G) nil ->
+ ok_LF (flat_map snd_ G) nil ->
  v \notin (used_w_vars G) ->
- ok (flat_map snd ((w, nil) :: G)) nil.
+ ok_LF (flat_map snd_ ((w, nil) :: G)) nil.
 Admitted. (* !!! *)
 
-Lemma ok_fresh_wo_te_list:
+Lemma ok_LF_fresh_wo_te_list:
 forall G v A w,
- ok G nil ->
+ ok_LF G nil ->
  w \notin (used_w_vars G) ->
- ok ((w, (v,A)::nil) :: G) nil.
+ ok_LF ((w, (v,A)::nil) :: G) nil.
 Admitted. (* !!! *)
 
-Lemma ok_fresh_wo_te_ty:
+Lemma ok_LF_fresh_wo_te_ty:
 forall G v A w,
- ok (flat_map snd G) nil ->
+ ok_LF (flat_map snd_ G) nil ->
  w \notin (used_w_vars G) ->
- ok (flat_map snd ((w, (v,A)::nil) :: G)) nil.
+ ok_LF (flat_map snd_ ((w, (v,A)::nil) :: G)) nil.
 Admitted. (* !!! *)
 
-Lemma ok_empty_first_list:
+Lemma ok_LF_empty_first_list:
 forall w G Gamma,
-  ok ((w,Gamma) :: G) nil ->
-  ok ((w, (@nil (prod var ty))) :: G) nil.
+  ok_LF ((w,Gamma) :: G) nil ->
+  ok_LF ((w, (@nil (prod var ty))) :: G) nil.
 Admitted. (* !!! *)
 
-Lemma ok_empty_first_ty:
+Lemma ok_LF_empty_first_ty:
 forall (w: var) G Gamma,
-  (@ok ty (flat_map snd ((w,Gamma) :: G)) nil) ->
-  (@ok ty (flat_map snd ((w, nil) :: G)) nil).
+  (@ok_LF ty (flat_map snd_ ((w,Gamma) :: G)) nil) ->
+  (@ok_LF ty (flat_map snd_ ((w, nil) :: G)) nil).
 Admitted. (* !!! *)
 
 (* ok_Bg *)
@@ -150,8 +192,8 @@ Admitted. (* !!! *)
 Add Morphism ok_Bg : ok_Bg_PPermut.
 intros; unfold ok_Bg; split; intros;
 destruct H0; split;
-[ rewrite <- H | eapply ok_PPermut_ty |
-  rewrite H | eapply ok_PPermut_ty; try symmetry ]; eauto.
+[ rewrite <- H | eapply ok_LF_PPermut_ty |
+  rewrite H | eapply ok_LF_PPermut_ty; try symmetry ]; eauto.
 Qed.
 
 Lemma ok_Bg_ppermut:
@@ -188,8 +230,8 @@ forall G Gamma v A w,
  v \notin (used_t_vars ((w,Gamma)::G)) ->
  ok_Bg ((w, (v,A)::Gamma) :: G).
 intros; unfold ok_Bg in *;  destruct H; split;
-[ apply ok_fresh_te_list |
-  apply ok_fresh_te_ty]; auto.
+[ apply ok_LF_fresh_te_list |
+  apply ok_LF_fresh_te_ty]; auto.
 Qed.
 
 Lemma ok_Bg_fresh_wo:
@@ -198,8 +240,8 @@ forall G w,
  w \notin (used_w_vars G) ->
  ok_Bg ((w, nil) :: G).
 intros; unfold ok_Bg in *;  destruct H; split;
-[ eapply ok_fresh_wo_list |
-  eapply ok_fresh_wo_ty]; eauto.
+[ eapply ok_LF_fresh_wo_list |
+  eapply ok_LF_fresh_wo_ty]; eauto.
 Qed.
 
 Lemma ok_Bg_fresh_wo_te:
@@ -208,8 +250,8 @@ forall G w v A,
  w \notin (used_w_vars G) ->
  ok_Bg ((w, (v, A) :: nil) :: G).
 intros; unfold ok_Bg in *;  destruct H; split;
-[ apply ok_fresh_wo_te_list |
-  apply ok_fresh_wo_te_ty]; eauto.
+[ apply ok_LF_fresh_wo_te_list |
+  apply ok_LF_fresh_wo_te_ty]; eauto.
 Qed.
 
 Lemma ok_Bg_cons_last:
@@ -236,22 +278,23 @@ forall G C C' w x A,
   ok_Bg ((w, C) :: G) ->
   C *=* (x,A)::C' ->
   ok_Bg ((w, C') :: G).
+(*
 intros;
 assert ((w,(x, A) :: C') :: G ~=~ (w, C) :: G) by PPermut_simpl;
-rewrite <- H1 in H; unfold ok_Bg in *; destruct H; split; simpl in *;
+rewrite <- H1 in H; unfold ok_Bg in *; destruct H; split; simpl in *.
 repeat case_if; auto;
-apply ok_used_weakening with (x:=x); auto.
-Qed.
+apply ok_LF_used_weakening with (x:=x); auto.
+Qed. *) Admitted.
 Hint Resolve ok_Bg_permut_first_tail : ok_bg_rew.
 
 Lemma ok_Bg_empty_first:
 forall w G Gamma,
   ok_Bg ((w,Gamma) :: G) ->
   ok_Bg ((w, nil) :: G).
-intros; unfold ok_Bg; destruct H; split;
-[eapply ok_empty_first_list |
- eapply ok_empty_first_ty]; eauto.
-Qed.
+(*intros; unfold ok_Bg; destruct H; split;
+[eapply ok_LF_empty_first_list |
+ eapply ok_LF_empty_first_ty]; eauto.
+Qed.*) Admitted.
 
 Hint Resolve ok_Bg_empty_first : ok_bg_rew.
 
@@ -261,18 +304,19 @@ forall w C C' v A A0 G,
   C *=* (v, A) :: C' ->
   Mem (v, A0) C ->
   A0 = A.
-intros; destruct (eq_ty_dec A0 A); auto;
+(*intros; destruct (eq_ty_dec A0 A); auto;
 assert (exists gh, exists gt, C' = gh & (v, A0) ++ gt) by
   ( apply permut_neq_split with (b := (v, A)) (l1 := C); auto;
     intro HH; inversion HH; subst; elim n; auto);
 destruct H2 as (gh); destruct H2 as (gt); subst;
 assert (C *=* (v, A) :: (v, A0) :: gh ++ gt) by (rewrite H0; permut_simpl);
 unfold ok_Bg in *; destruct H;
-assert (ok (flat_map snd ((w, (v, A) :: (v, A0) :: gh ++ gt ) :: G )) nil) by
-  (apply ok_PPermut_ty with (G := ((w, C) :: G)); [PPermut_simpl | auto]);
+assert (ok_LF (flat_map snd_ ((w, (v, A) :: (v, A0) :: gh ++ gt ) :: G )) nil)
+by
+  (apply ok_LF_PPermut_ty with (G := ((w, C) :: G)); [PPermut_simpl | auto]);
 simpl in *; repeat case_if;
 elim H6; apply Mem_here.
-Qed.
+Qed.*) Admitted.
 
 Lemma ok_Bg_Mem_contradict:
 forall A A' w w' v C C' G G',
@@ -280,7 +324,7 @@ forall A A' w w' v C C' G G',
  Mem (v, A) C ->
  G ~=~ G' & (w', (v, A') :: C') ->
  False.
-intros.
+(*intros.
 rewrite H1 in H.
 apply permut_Mem_split_head with (l2 := C) in H0; auto;
 destruct H0 as (gh); destruct H0 as (gt); subst.
@@ -288,11 +332,15 @@ assert ((w, gh & (v, A) ++ gt) :: G' & (w', (v, A') :: C') ~=~
         (w, (v, A) :: gh ++ gt) :: (w', (v, A') :: C') :: G') by
 (PPermut_simpl; apply PPermut_skip; [permut_simpl | auto]).
 rewrite H0 in H; unfold ok_Bg in H; destruct H.
+rew_flat_map in *. simpl ok_LF in H2.
 simpl in *; repeat case_if.
-assert (ok ((v, A') :: C' ++ flat_map snd G') (v :: nil)).
-  eapply ok_split with (G1:=gh++gt). (* exact H2.  ?!? *) skip. (* !!! *)
+assert (ok_LF ((v, A') :: C' ++ flat_map snd_ G') (v :: nil)).
+  eapply ok_LF_split with (G1:=flat_map snd_ ((w, gh++gt)::nil)).
+simpl. simpl in H2. rew_flat_map in H2. simpl in H2.
+simpl; rew_app. simpl in H2; case_if.
+(* exact H2.  ?!? *) skip. (* !!! *)
 simpl in H6; case_if; elim H7; apply Mem_here.
-Qed.
+Qed.*) Admitted.
 
 Lemma ok_Bg_permut_no_last:
 forall G w C v A,
@@ -313,15 +361,15 @@ Lemma ok_Bg_no_last:
 forall G w C,
   ok_Bg (G & (w,C)) ->
   ok_Bg G.
-intros. assert (G & (w,C) ~=~ ((w, C) :: nil) ++ G) by PPermut_simpl;
+(*intros. assert (G & (w,C) ~=~ ((w, C) :: nil) ++ G) by PPermut_simpl;
 rewrite H0 in H;
 destruct H; split.
 eapply ok_split in H; destruct H; auto.
 simpl in H1.
-assert (ok C nil /\ ok (flat_map snd G) nil) by skip. (* !!! *)
-  (* eapply ok_split with (A:= var) (G1:=C) (G2:=flat_map snd G) (U:=nil). *)
+assert (ok_LF C nil /\ ok_LF (flat_map snd_ G) nil) by skip. (* !!! *)
+  (* eapply ok_split with (A:= var) (G1:=C) (G2:=flat_map snd_ G) (U:=nil). *)
 destruct H2; auto.
-Qed.
+Qed.*) Admitted.
 Hint Resolve ok_Bg_no_last.
 
 Lemma ok_Bg_permut_no_last_spec2:
@@ -344,8 +392,8 @@ forall w w' C C' G,
 intros.
 assert ((w, C) :: G & (w', C') ~=~ (w, C) :: (w', C') :: G) by PPermut_simpl;
 rewrite H0 in H;
-destruct H; simpl in *; repeat case_if.
-intro; elim H3; rewrite Mem_cons_eq; left; symmetry; auto.
+destruct H; simpl in *. inversion H; subst; inversion H7; subst.
+rewrite Mem_cons_eq in H8. rewrite Mem_nil_eq in H8. auto.
 Qed.
 
 Lemma ok_Bg_last_last2_neq:
@@ -355,15 +403,15 @@ forall w w' C C' G,
 intros;
 assert (G & (w, C) & (w', C') ~=~ (w, C) :: (w', C') :: G) by PPermut_simpl;
 rewrite H0 in H;
-destruct H; simpl in *; repeat case_if.
-intro; elim H3; rewrite Mem_cons_eq; left; symmetry; auto.
+destruct H; simpl in *; inversion H; subst; inversion H7; subst.
+rewrite Mem_cons_eq in H8. rewrite Mem_nil_eq in H8; auto.
 Qed.
 
 Lemma ok_Bg_swap_worlds:
 forall G w w' C C',
   ok_Bg (G & (w, C) & (w', C')) ->
   ok_Bg (G & (w', C) & (w, C')).
-intros.
+(*intros.
 assert (G & (w, C) & (w', C') ~=~ (w, C) :: (w', C') :: G) by PPermut_simpl.
 rewrite H0 in H.
 assert (G & (w', C) & (w, C') ~=~ (w', C) :: (w, C') :: G) by PPermut_simpl.
@@ -374,7 +422,7 @@ rewrite Mem_cons_eq in H4; elim H6; destruct H4; subst;
 [ apply Mem_here | rewrite Mem_nil_eq in H4; contradiction].
 apply ok_used_permut with (U := w'::w::nil); [permut_simpl | ]; auto.
 auto.
-Qed.
+Qed. *) Admitted.
 
 Lemma ok_Bg_impl_ppermut:
 forall G G' w C C',
@@ -393,32 +441,32 @@ Lemma ok_Bg_split1:
 forall G w w' C C',
   ok_Bg ((w,C)::G & (w',C')) ->
   ok_Bg ((w, C ++ C') :: G).
-intros.
+(*intros.
 assert ((w, C) :: G & (w', C') ~=~ (w,C) :: (w', C')::G) by PPermut_simpl.
 rewrite H0 in H; destruct H; split; simpl in *;
 repeat case_if.
 apply ok_used_weakening with (x:=w'); auto.
 skip. (* this should be rew_app; auto *)
-Qed.
+Qed.*) Admitted.
 
 Lemma ok_Bg_split2:
 forall G w w' C C',
   ok_Bg ((w,C)::G & (w',C')) ->
   ok_Bg ((w', C' ++ C) :: G).
-intros.
+(*intros.
 assert ((w, C) :: G & (w', C') ~=~ (w', C') :: (w, C)::G) by PPermut_simpl.
 rewrite H0 in H; destruct H; split; simpl in *;
 repeat case_if.
 rewrite Mem_nil_eq in H2; auto.
 apply ok_used_weakening with (x:=w); auto.
 skip. (* this should be rew_app; auto *)
-Qed.
+Qed. *) Admitted.
 
 Lemma ok_Bg_split3:
 forall G w w' w'' C C' C'',
   ok_Bg ((w,C)::G & (w',C') & (w'',C'')) ->
   ok_Bg ((w, C) :: G & (w', C' ++ C'')).
-intros.
+(*intros.
 assert ((w, C) :: G & (w', C') & (w'',C'') ~=~
   (w, C) :: (w', C'):: (w'',C'') :: G) by PPermut_simpl.
 assert ((w,C) :: G & (w', C'++C'') ~=~ (w,C) :: (w', C'++C'') :: G)
@@ -427,13 +475,13 @@ rewrite H0 in H; rewrite H1; destruct H; split; simpl in *;
 repeat case_if.
 apply ok_used_weakening with (x:=w''); auto.
 skip. (* this should be rew_app; auto *)
-Qed.
+Qed. *) Admitted.
 
 Lemma ok_Bg_split4:
 forall G w w' C C',
   ok_Bg (G & (w, C) & (w', C')) ->
   ok_Bg (G & (w', C' ++ C)).
-intros.
+(*intros.
 assert (G & (w, C) & (w', C') ~=~
   (w, C) :: (w', C') :: G) by PPermut_simpl.
 assert (G & (w', C'++C) ~=~ (w', C'++C) :: G)
@@ -445,13 +493,13 @@ apply ok_used_weakening with (x:=w);
 apply ok_used_permut with (U:= w'::w::nil).
 permut_simpl. auto.
 skip. (* this should be rew_app; auto *)
-Qed.
+Qed. *) Admitted.
 
 Lemma ok_Bg_split5:
 forall G w w' C C',
   ok_Bg (G & (w, C) & (w', C')) ->
   ok_Bg (G & (w, C ++ C')).
-intros.
+(* intros.
 assert (G & (w, C) & (w', C') ~=~
   (w, C) :: (w', C') :: G) by PPermut_simpl.
 assert (G & (w, C++C') ~=~ (w, C++C') :: G)
@@ -460,13 +508,13 @@ rewrite H0 in H; rewrite H1; destruct H; split; simpl in *;
 repeat case_if.
 apply ok_used_weakening with (x:=w'); auto.
 skip. (* this should be rew_app; auto *)
-Qed.
+Qed. *) Admitted.
 
 Lemma ok_Bg_split6:
 forall G w C C' C'' w' w'',
   ok_Bg (G & (w, C) & (w', C') & (w'', C'')) ->
   ok_Bg (G & (w, C ++ C') & (w'', C'')).
-intros.
+(*intros.
 assert (G & (w,C) & (w', C') & (w'',C'') ~=~
   (w, C) :: (w', C'):: (w'',C'') :: G) by PPermut_simpl.
 assert (G & (w, C++C') & (w'', C'') ~=~ (w, C ++ C') :: (w'', C'') :: G)
@@ -481,7 +529,7 @@ apply ok_used_permut with (U:= w''::w'::w::nil).
   permut_simpl.
   auto.
 skip. (* this should be rew_app; auto *)
-Qed.
+Qed. *) Admitted.
 
 (* This is actually false
 Lemma ok_Bg_split7:
@@ -494,7 +542,7 @@ Lemma ok_Bg_split8:
 forall G G' w w' w'' C C' C'',
   ok_Bg (G ++ G' ++ (w, C) :: (w', C') :: (w'', C'') :: nil) ->
   ok_Bg (G ++ G' ++ (w', C') :: (w'', C'' ++ C)::nil) .
-intros.
+(*intros.
 assert (G++G' ++ (w, C) :: (w', C') :: (w'',C'') :: nil ~=~
   (w, C) :: (w', C'):: (w'',C'') :: G ++ G') by PPermut_simpl.
 assert (G ++ G' ++ (w', C') :: (w'', C'' ++ C) :: nil ~=~
@@ -510,13 +558,13 @@ apply ok_used_weakening with (x:=w);
 apply ok_used_permut with (U:=w'' :: w' :: w :: nil);
 auto; permut_simpl.
 skip. (* this should be rew_app; permut; auto *)
-Qed.
+Qed. *) Admitted.
 
 Lemma ok_Bg_split9:
 forall G w w' w'' C C' C'',
   ok_Bg ((w,C)::G & (w',C') & (w'',C'')) ->
   ok_Bg ((w, C++C') :: G & (w'', C'')).
-intros.
+(*intros.
 assert ((w, C) :: G & (w', C') & (w'',C'') ~=~
   (w, C) :: (w', C'):: (w'',C'') :: G) by PPermut_simpl.
 assert ((w, C++C') :: G & (w'', C'')  ~=~
@@ -531,13 +579,13 @@ apply ok_used_weakening with (x:=w');
 apply ok_used_permut with (U:=w'' :: w' :: w :: nil);
 auto; permut_simpl.
 skip. (* this should be rew_app; permut; auto *)
-Qed.
+Qed. *) Admitted.
 
 Lemma ok_Bg_split10:
 forall G G' w1 w2 w3 w4 c1 c2 c3 c4,
   ok_Bg (G ++ (w1, c1)::G' ++ (w2, c2) :: (w3, c3) :: (w4, c4) :: nil) ->
   ok_Bg (G ++ (w1, c1)::G' ++ (w2, c2 ++ c3) :: (w4, c4) :: nil).
-intros.
+(*intros.
 assert (G ++ (w1,c1) :: G' ++ (w2, c2) :: (w3, c3) :: (w4,c4) :: nil ~=~
    (w1,c1) :: (w2, c2) :: (w3, c3) :: (w4,c4) :: G ++ G') by PPermut_simpl.
 assert (G ++ (w1, c1) :: G' ++ (w2, c2 ++ c3) :: (w4, c4) :: nil~=~
@@ -554,7 +602,7 @@ apply ok_used_weakening with (x:=w3);
 apply ok_used_permut with (U:=w4 :: w3 :: w2 :: w1 :: nil);
 auto; permut_simpl.
 skip. (* this should be rew_app; permut; auto *)
-Qed.
+Qed. *) Admitted.
 
 Hint Resolve ok_Bg_split1 ok_Bg_split2 ok_Bg_split3 ok_Bg_split4
   ok_Bg_split5 ok_Bg_split6 ok_Bg_split8
@@ -567,14 +615,15 @@ Hint Resolve ok_Bg_swap_worlds.
 Lemma ok_Bg_skip_last:
 forall G C,
   ok_Bg (G & C) -> ok_Bg G.
+(*
 intros;
 assert (G & C ~=~ (C :: nil) ++ G) by PPermut_simpl; rewrite H0 in H;
 destruct H; split.
-eapply ok_split with (G1:=C::nil) (G2:=G); eauto.
-simpl in *; destruct C; case_if.
-eapply ok_split with (G1:=snd (v,l)) (G2:=flat_map snd  G); auto.
+eapply ok_LF_split with (G1:=C::nil) (G2:=G); eauto.
+simpl in *; destruct C. case_if.
+eapply ok_split with (G1:=snd_ (v,l)) (G2:=flat_map snd_  G); auto.
 skip. (* exact H1 *)
-Qed.
+Qed. *) Admitted.
 
 Hint Resolve ok_Bg_skip_last: ok_bg_rew.
 
